added callstate matching up to cmajor

src/Cmajor.v
@@ -288,8 +288,14 @@ Inductive step: state -> trace -> state -> Prop :=
 
 End RELSEM.
 
-Inductive is_callstate (p : program) : value -> value -> state -> Prop := .
-(* TODO: stub *)
+Inductive is_callstate (p : program) : value -> value -> state -> Prop := 
+| IsCallstate :
+    forall fname vs arg fb fofs argptr m fn,
+      value_inject (Genv.globalenv p) m (Close fname vs) (Vptr fb fofs) ->
+      value_inject (Genv.globalenv p) m arg argptr ->
+      Genv.find_funct_ptr (Genv.globalenv p) fb = Some fn ->
+      Genv.find_symbol (Genv.globalenv p) fname = Some fb ->
+      is_callstate p (Close fname vs) arg (Callstate fn ((Vptr fb fofs) :: argptr :: nil) Kstop m).
 
 (** A final state is a [Returnstate] with an empty continuation. *)
 
@@ -330,8 +336,16 @@ Inductive cminor_final_state(p : Cminor.program): Cminor.state -> value -> Prop 
     value_inject (Genv.globalenv p) m v v' ->
     cminor_final_state p (Cminor.Returnstate v' Cminor.Kstop m) v.
 
-Inductive cminor_is_callstate (p : Cminor.program) : value -> value -> state -> Prop := .
-(* TODO: stub *)
+Inductive cminor_is_callstate (p : Cminor.program) : value -> value -> state -> Prop := 
+| CmIsCallstate :
+    forall fname vs arg fb fofs argptr m fn,
+      value_inject (Genv.globalenv p) m (Close fname vs) (Vptr fb fofs) ->
+      value_inject (Genv.globalenv p) m arg argptr ->
+      Genv.find_funct_ptr (Genv.globalenv p) fb = Some fn ->
+      Genv.find_symbol (Genv.globalenv p) fname = Some fb ->
+      cminor_is_callstate p (Close fname vs) arg (Callstate fn ((Vptr fb fofs) :: argptr :: nil) Kstop m).
+
 
 Definition Cminor_semantics (p: Cminor.program) :=
   Semantics Cminor.step (cminor_is_callstate p) (cminor_final_state p) (Genv.globalenv p).
+
